cfg/CncLoop.v
@@ -1,0 +1,22 @@
+Require Export CFGinnermost.
+
+(** cnc & ocnc **)
+
+Definition cnc_loop `{C : redCFG} s q s'
+  := loop_contains s' s /\ ~ deq_loop q s'.
+
+Definition ocnc_loop `{C : redCFG} s q s'
+  := cnc_loop s q s' /\ forall x, cnc_loop s q s' -> deq_loop x s'.
+
+(* the ocnc loop has an exit such that q is deeper or equal to the exit *)
+Lemma ocnc_loop_exit `(C : redCFG) s q s'
+      (Hocnc : ocnc_loop s q s')
+  : exists e : Lab, exited s' e /\ deq_loop q e.
+Admitted.
+
+Lemma ex_ocnc_loop `(C : redCFG) s q
+      (Hndeq : ~ deq_loop q s)
+      (Hsdeq : deq_loop s q) (* <-- is this assumption really necessary ? *)
+  : exists s', ocnc_loop s q s'.
+Admitted.
+ 
